MirrorCharge!/src/MirrorCharge/Imp/NonRefl_NoMem_Skips.v
@@ -1,0 +1,69 @@
+Require Import Coq.Strings.String.
+Require Import ExtLib.Structures.Applicative.
+Require Import ExtLib.Data.Fun.
+Require Import Charge.Logics.ILogic.
+Require Import Charge.Logics.BILogic.
+Require Import Charge.Logics.ILEmbed.
+Require Import Charge.Logics.ILInsts.
+Require Import Charge.Logics.BILInsts.
+Require Import MirrorCharge.Imp.Imp.
+Require Import MirrorCharge.Imp.Goal.
+
+Local Open Scope string_scope.
+
+Local Existing Instance ILogicOps_HProp.
+Local Existing Instance ILogic_HProp.
+Local Existing Instance BILogicOps_HProp.
+Local Existing Instance ILogicOps_SProp.
+Local Existing Instance ILogic_SProp.
+Local Existing Instance BILogicOps_SProp.
+Local Existing Instance ILogicOps_lprop.
+Local Existing Instance ILogic_lprop.
+Local Existing Instance BILOps.
+Local Existing Instance BILogic.
+Local Existing Instance EmbedOp_Prop_HProp.
+Local Existing Instance Embed_Prop_HProp.
+Local Existing Instance EmbedOp_HProp_lprop.
+Local Existing Instance Embed_HProp_lprop.
+Local Existing Instance EmbedOp_Prop_SProp.
+Local Existing Instance Embed_Prop_SProp.
+
+Ltac verify :=
+  repeat first [ apply triple_exL ; apply lforallR ; intro
+               | apply Skip_seq_rule
+               | apply Assign_seq_rule
+               | apply Skip_tail_rule
+               | apply Assign_tail_rule
+               | apply Skip_tail_rule ].
+
+Goal ltrue |-- triple ltrue (skips 5) ltrue.
+Proof.
+unfold skips.
+Time verify.
+eapply embed_ltrue.
+eapply ltrueR.
+Time Qed.
+
+Goal ltrue |-- triple ltrue (skips 10) ltrue.
+Proof.
+unfold skips.
+Time verify.
+eapply embed_ltrue.
+eapply ltrueR.
+Time Qed.
+
+Goal ltrue |-- triple ltrue (skips 15) ltrue.
+Proof.
+unfold skips.
+Time verify.
+eapply embed_ltrue.
+eapply ltrueR.
+Time Qed.
+
+Goal ltrue |-- triple ltrue (skips 20) ltrue.
+Proof.
+unfold skips.
+Time verify.
+eapply embed_ltrue.
+eapply ltrueR.
+Time Qed.
